@base <https://web-payments.org/vocabs/commerce> .
@prefix dcterms: <http://purl.org/dc/terms/> .
@prefix owl: <http://www.w3.org/2002/07/owl#> .
@prefix rdf: <http://www.w3.org/1999/02/22-rdf-syntax-ns#> .
@prefix rdfs: <http://www.w3.org/2000/01/rdf-schema#> .
@prefix schema: <http://schema.org/> .
@prefix xhv: <http://www.w3.org/1999/xhtml/vocab#> .
@prefix xsd: <http://www.w3.org/2001/XMLSchema#> .

<https://w3id.org/commerce#Account> a rdfs:Class;
   rdfs:label "Account"@en;
   rdfs:comment """
A financial device that can operate as a source or destination for funds 
transfered during a commercial exchange.
          """@en;
   rdfs:subclassOf rdfs:Class;
   <vs:term_status> "unstable"@en .

<https://w3id.org/commerce#Deposit> a rdfs:Class;
   rdfs:label "Deposit"@en;
   rdfs:comment """
A transfer of funds from a source account into a destination account typically
performed as a means for storing monetary amounts in the destination account.
          """@en;
   rdfs:subclassOf <https://w3id.org/commerce#Transaction>;
   <vs:term_status> "unstable"@en .

<https://w3id.org/commerce#Payee> a rdfs:Class;
   rdfs:label "Payee"@en;
   rdfs:comment """
An entity that defines how monetary funds should be transferred to a destination 
account during a Transaction. A list of Payees can be 
processed to produce a list of Transfers.
          """@en;
   <vs:term_status> "unstable"@en .

<https://w3id.org/commerce#PayeeRule> a rdfs:Class;
   rdfs:label "PayeeRule"@en;
   rdfs:comment """
A Payee Rule is a mechanism that can describe limits and allowances on the 
payees during a transaction. These rules are typically used to apply 
algorithmic formulas to the final price of a particular good. For example,
minimum and maximum prices, tax rates, when taxes are applied, and preventing
additional payees are a few examples of the types of payee rules that can be
specified using PayeeRules.
          """@en;
   rdfs:subclassOf rdfs:Class;
   <vs:term_status> "unstable"@en .

<https://w3id.org/commerce#Transaction> a rdfs:Class;
   rdfs:label "Transaction"@en;
   rdfs:comment """
A record of a commercial exchange between two entities resulting in the 
transfer of monetary funds from one or more source accounts to 
one or more destination accounts.
          """@en;
   rdfs:subclassOf rdfs:Class;
   <vs:term_status> "unstable"@en .

<https://w3id.org/commerce#Transfer> a rdfs:Class;
   rdfs:label "Transfer"@en;
   rdfs:comment """
A record of the movement of monetary funds from a source account into a
destination account.
          """@en;
   rdfs:subclassOf rdfs:Class;
   <vs:term_status> "unstable"@en .

<https://w3id.org/commerce#Withdrawal> a rdfs:Class;
   rdfs:label "Withdrawal"@en;
   rdfs:comment """
A transfer of funds from a source account into a destination account typically
performed as a means for retrieving previously stored monetary amounts.
          """@en;
   rdfs:subclassOf <https://w3id.org/commerce#Transaction>;
   <vs:term_status> "unstable"@en .

<https://w3id.org/commerce> a owl:Ontology;
   rdfs:label "Commerce Vocabulary"@en;
   dcterms:abstract """Abstract
      
This document describes a number of classes and properties that can be used to
express commercial transactions using Linked Data on the Web. These include 
things such as deposits, withdrawals, how entities should be paid for goods or
services rendered, receipts, payment details, and digital signatures on 
financial transactions.
      
    """@en;
   rdfs:comment """
This document describes a number of classes and properties that can be used to
express commercial transactions using Linked Data on the Web. These include 
things such as deposits, withdrawals, how entities should be paid for goods or
services rendered, receipts, payment details, and digital signatures on 
financial transactions.
      """@en .

<https://w3id.org/commerce#Cumulative> a rdf:Property;
   rdfs:label "Cumulative"@en;
   rdfs:comment """
This constant term is used to specify a cumulative rate context in a Payee. 
Normally a percentage-based Payee's amount would be calculated by applying its 
percentage rate to the total of all flat amount Payees from the Payee list. By 
specifying that a Payee uses cumulative rate context, the total amount will also 
include amounts calculated for other percentage-based Payees that appear in 
positions prior to the Payee with the cumulative rate context. Therefore, the 
more ExclusivePercentage Payees that appear before a cumulative Payee, the 
larger the total will be that the percentage is applied to in order to calculate 
its amount.
        """@en;
   <vs:term_status> "unstable"@en .

<https://w3id.org/commerce#Deferred> a rdf:Property;
   rdfs:label "Deferred"@en;
   rdfs:comment """
This constant term is used to specify a deferred rate context. A deferred
rate context specifies that the amount of a percentage-based Payee must be 
calculated after all non-deferred Payee amounts have already been calculated. 
This is most useful when a Payee should be applied to the total cost of a good 
or service. Whilst Payees that are Taxes are automatically deferred, if a Payee 
that is not a Tax wishes to behave like one, it should use this rate context.
        """@en;
   <vs:term_status> "unstable"@en .

<https://w3id.org/commerce#ExclusivePercentage> a rdf:Property;
   rdfs:label "ExclusivePercentage"@en;
   rdfs:comment """
This constant term is used to specify an exclusive percentage-based rate type.
An exclusive percentage-based rate type specifies that the rate is a percentage
and the percentage should be applied to the total price of all payees that are
not also percentage-based. There are some exceptions to this rule when using a 
cumulative rate context (see: Cumulative). The amount that results from this 
percentage will be added to the total amount calculated from all of the Payees. 
This behavior is the opposite of that of an InclusivePercentage, where the total 
would not be altered. Real world examples of ExclusivePercentages include most 
sales taxes in the United States.
        """@en;
   <vs:term_status> "unstable"@en .

<https://w3id.org/commerce#FlatAmount> a rdf:Property;
   rdfs:label "FlatAmount"@en;
   rdfs:comment """
A flat amount rate type expresses that a payment amount is a specific amount
in a given currency. That is, the rate is to be interpreted as a fixed amount,
not as a percentage.
        """@en;
   <vs:term_status> "unstable"@en .

<https://w3id.org/commerce#InclusivePercentage> a rdf:Property;
   rdfs:label "InclusivePercentage"@en;
   rdfs:comment """
This constant term is used to specify an inclusive percentage-based rate type.
An inclusive percentage-based rate type specifies that the rate is a percentage
and the percentage should be applied to the total price of all payees that are
not also percentage-based. There are some exceptions to this rule when using 
a cumulative rate context (see: Cumulative). The amount that results from 
this percentage will be evenly deducted from all other Payees, thus leaving 
the total the same. This behavior is the opposite of that of an 
ExclusivePercentage, where the amount would be added to the total and the 
other Payees would remain the same. Real world examples of InclusivePercentages 
include most income taxes in the United States.
        """@en;
   <vs:term_status> "unstable"@en .

<https://w3id.org/commerce#Tax> a rdf:Property;
   rdfs:label "Tax"@en;
   rdfs:comment """
This constant specifies that the Payee's rate specified is a tax.
        """@en;
   <vs:term_status> "unstable"@en .

<https://w3id.org/commerce#TaxExempt> a rdf:Property;
   rdfs:label "TaxExempt"@en;
   rdfs:comment """
This constant specifies that a payment to the Payee should not have any
taxes collected for the transfer of funds. Typically, these Payees are 
non-profit corporations or other organizations that are under a non-taxable
status.
        """@en;
   <vs:term_status> "unstable"@en .

<https://w3id.org/commerce#account> a rdf:Property;
   rdfs:label "account"@en;
   rdfs:comment """
The account property specifies a resource that is used to keep track of
economic value that is under the control of a particular entity.
        """@en;
   rdfs:domain schema:Thing;
   rdfs:range <https://w3id.org/commerce#Account>;
   <vs:term_status> "unstable"@en .

<https://w3id.org/commerce#amount> a rdf:Property;
   rdfs:label "amount"@en;
   rdfs:comment """
The amount property is used to specify the total value of a financial
resource or action such as an account, transfer, or transaction.
        """@en;
   rdfs:domain schema:Thing;
   rdfs:range rdfs:Literal;
   <vs:term_status> "unstable"@en .

<https://w3id.org/commerce#currency> a rdf:Property;
   rdfs:label "currency"@en;
   rdfs:comment """
The currency property is used to specify the monetary system that is used when
specifying the financial amount of a commercial exchange. The value SHOULD 
be an ISO-4217 currency or a dereference-able IRI to a monetary system that 
is not specified in ISO-4217.
        """@en;
   rdfs:domain schema:Thing;
   rdfs:range rdfs:Resource;
   <vs:term_status> "unstable"@en .

<https://w3id.org/commerce#date> a rdf:Property;
   rdfs:label "date"@en;
   rdfs:comment """
The date property specifies the date and time on which a commercial transaction 
occurred. The value MUST be expressed using an ISO-8601 date/time string.
        """@en;
   rdfs:domain schema:Event;
   rdfs:range xsd:dateTime;
   <vs:term_status> "unstable"@en .

<https://w3id.org/commerce#destination> a rdf:Property;
   rdfs:label "destination"@en;
   rdfs:comment """
This property is used to specify a destination account for a commercial 
transaction.
        """@en;
   rdfs:domain schema:Thing;
   rdfs:range <https://w3id.org/commerce#Account>;
   <vs:term_status> "unstable"@en .

<https://w3id.org/commerce#destinationOwnerType> a rdf:Property;
   rdfs:label "destinationOwnerType"@en;
   rdfs:comment """
Specifies the type of the destination account, typically used in a PayeeRule 
where the type of destination account payment is to be restricted.
        """@en;
   rdfs:domain schema:Thing;
   rdfs:range schema:Thing;
   <vs:term_status> "unstable"@en .

<https://w3id.org/commerce#forTransaction> a rdf:Property;
   rdfs:label "forTransaction"@en;
   rdfs:comment """
This property is most often used to specify that a Transfer is for the
specified Transaction. The relationship from Transaction to Transfer is 
encoded using the transfer property. The relationship 
from Transfer to Transaction is encoded using this property.
        """@en;
   rdfs:domain <https://w3id.org/commerce#Transfer>;
   rdfs:range <https://w3id.org/commerce#Transaction>;
   <vs:term_status> "unstable"@en .

<https://w3id.org/commerce#gatewayApprovalCode> a rdf:Property;
   rdfs:label "gatewayApprovalCode"@en;
   rdfs:comment """
The gateway approval code is typically used to express the result of a credit
card processing gateway. These codes are typically a string that is specific to
the processing gateway software.
        """@en;
   rdfs:domain schema:Thing;
   rdfs:range rdfs:Literal;
   <vs:term_status> "unstable"@en .

<https://w3id.org/commerce#gatewayError> a rdf:Property;
   rdfs:label "gatewayError"@en;
   rdfs:comment """
The gateway error is typically used to encode an error that occurred when
processing a credit card or debit card. An error code is typically a string
that is specific to the processing gateway software.
        """@en;
   rdfs:domain schema:Thing;
   rdfs:range rdfs:Literal;
   <vs:term_status> "unstable"@en .

<https://w3id.org/commerce#limitation> a rdf:Property;
   rdfs:label "limitation"@en;
   rdfs:comment """
This property is often used with a PayeeRule and expresses a restriction on 
a Payee. For example, a PayeeRule may provide restrictions on the type of a 
Payee or the amounts that Payee may receive as a participant in a commercial 
transaction.
        """@en;
   rdfs:domain schema:Thing;
   rdfs:range rdfs:Resource;
   <vs:term_status> "unstable"@en .

<https://w3id.org/commerce#maximumRate> a rdf:Property;
   rdfs:label "maximumRate"@en;
   rdfs:comment """
This property is typically used in a PayeeRule to limit the maximum rate that
a Payee can receive as a part of a transaction. These types of rules ensure that
no single Payee can capture more of the final sale price than the asset owner 
is willing to give up. Maximum rate limitations allow statements like the
following: "I want to limit the amount of money that a payment gateway
can collect to less than 4%".
        """@en;
   rdfs:domain schema:Thing;
   rdfs:range rdfs:Literal;
   <vs:term_status> "unstable"@en .

<https://w3id.org/commerce#minimumAmount> a rdf:Property;
   rdfs:label "minimumAmount"@en;
   rdfs:comment """
This property is typically used in a Payee to express a minimum amount that
a Payee MUST receive as a part of a transaction. These types of rules ensure 
that a floor is set for a particular percentage-based Payee. Minimum amount 
claims enable statement like the following to be made: "I want 2% of the sale
or $0.02 USD, whichever is greater".
        """@en;
   rdfs:domain schema:Thing;
   rdfs:range rdfs:Literal;
   <vs:term_status> "unstable"@en .

<https://w3id.org/commerce#payee> a rdf:Property;
   rdfs:label "payee"@en;
   rdfs:comment """
This property is used to specify an entity that should be paid, or
has been paid, as a result of a commercial exchange. 
        """@en;
   rdfs:domain schema:Thing;
   rdfs:range <https://w3id.org/commerce#Payee>;
   <vs:term_status> "unstable"@en .

<https://w3id.org/commerce#payeePosition> a rdf:Property;
   rdfs:label "payeePosition"@en;
   rdfs:comment """
This property is used to coerce a set of Payees into an ordered list. The
order in which Payees are evaluated is vital to the final amount and 
Transfer list that is generated by processing the list of Payees.
        """@en;
   rdfs:domain schema:Thing;
   rdfs:range rdfs:Literal;
   <vs:term_status> "unstable"@en .

<https://w3id.org/commerce#paymentGateway> a rdf:Property;
   rdfs:label "paymentGateway"@en;
   rdfs:comment """
This property is used to specify the payment gateway. The gateway is typically
a string and is used by the transaction processing software to process payments
via credit card or debit card. 
        """@en;
   rdfs:domain schema:Thing;
   rdfs:range rdfs:Literal;
   <vs:term_status> "unstable"@en .

<https://w3id.org/commerce#rate> a rdf:Property;
   rdfs:label "rate"@en;
   rdfs:comment """
This property can be used to specify the fixed amount or a percentage-based
rate of a Payee. The rate specifies the amount that the Payee should be or
has been paid as a result of a commercial exchange.
        """@en;
   rdfs:domain schema:Thing;
   rdfs:range rdfs:Literal;
   <vs:term_status> "unstable"@en .

<https://w3id.org/commerce#rateContext> a rdf:Property;
   rdfs:label "rateContext"@en;
   rdfs:comment """
The rate context is used to specify at which point in a payment calculation 
a rate should apply. It allows Payees to be deferred until the end of 
payment calculation, or for Payees to be marked as Tax or TaxDeferred.
        """@en;
   rdfs:domain schema:Thing;
   rdfs:range rdfs:Resource;
   <vs:term_status> "unstable"@en .

<https://w3id.org/commerce#rateType> a rdf:Property;
   rdfs:label "rateType"@en;
   rdfs:comment """
The rate type property is used to specify whether the rate property of a
Payee is a fixed amount, an inclusive percentage or an exclusive percentage.
The rateType coupled with the currency, and rate specifies the exact 
monetary amount or calculation that must be employed during the final cost
calculation among a list of Payees.
        """@en;
   rdfs:domain schema:Thing;
   rdfs:range rdfs:Resource;
   <vs:term_status> "unstable"@en .

<https://w3id.org/commerce#source> a rdf:Property;
   rdfs:label "source"@en;
   rdfs:comment """
This property is used to specify a source account for a commercial 
transaction.
        """@en;
   rdfs:domain schema:Thing;
   rdfs:range <https://w3id.org/commerce#Account>;
   <vs:term_status> "unstable"@en .

<https://w3id.org/commerce#transfer> a rdf:Property;
   rdfs:label "transfer"@en;
   rdfs:comment """
This property is used to associate the commercial transfer of monetary funds 
during a Transaction. A list of transfers associated with a Transaction is the
complete record of the monetary funds, the source accounts and the destination
accounts for a particular Transaction.
        """@en;
   rdfs:domain schema:Thing;
   rdfs:range <https://w3id.org/commerce#Transfer>;
   <vs:term_status> "unstable"@en .

